\documentclass{article}

\begin{document}

\title{Exercise 2.3-3}
\author{Jack Maney}
\maketitle

Reformulating the problem slightly, we wish to prove that for all $n\geq 1$, if

\[
	T(2^n) = \left\{
		\begin{array}{lr}
			2 & \textrm{ if } n = 1 \\
			2 T(2^{n-1}) + 2^n & \textrm{ if } n > 1
		\end{array}
	\right.
\]

\noindent then $T(2^n) = 2^n lg(2^n) = n 2^n$.

First, if $n=1$, then $T(2) = 2 = 1 * 2^1$.

Suppose that $T(2^n) = n 2^n$ for some $n\geq 1$, and consider $T(2^{n+1})$. Since $n+1 > 1$, we have

\[
	T(2^{n+1}) = 2 T(2^n) + 2^{n+1} = 2n2^n + 2^{n+1} = n 2^{n+1} + 2^{n+1} = (n+1)2^{n+1}.
\]

Therefore, by induction, $T(2^n) = n2^n$ for all $n\geq 1$.



\end{document}