\documentclass{article}

\begin{document}

\title{Exercise 2.2-3}
\author{Jack Maney}
\maketitle

Assuming that we're searching a list $l$ for an element $v$, and assume that the probability of any element in $l$ equaling $v$ is $\frac{1}{n}$ (where $l$ has $n$ elements). Let $X$ be the random variable denoting the number of elements of $l$ that needs to be searched to find $v$ via linear search. Then, we have

\[
	E(X) = \sum\limits_{i=1}^n i P(X=i) = 1 \cdot \frac{1}{n} + \sum\limits_{i=2}^n i P(\textrm{the first } i-1 \textrm{ elements of } l \textrm{ are not } v)
\]
\[
	= \frac{1}{n} + \sum\limits_{i=2}^n i \left(1 - \frac{1}{n}\right)^{i-1}.
\]

Now, consider the polynomial $f(x) = \sum\limits_{i=2}^{n} i (1-x)^{i-1}$. We have,

\[
	\int f(x) dx = C - \sum\limits_{i=2}^n (1-x)^i = C + 1 + x - \sum\limits_{i=0}^n (1-x)^i 
\]
\[
	= C + 1 + x - \frac{1 - (1-x)^{n+1}}{1 - (1-x)} = C + 1 + x - \frac{ 1 - (1-x)^{n + 1}}{x}
\]

\noindent (for $x\not=0$, obviously).

Thus,

\[
	f(x) = \frac{d}{dx}\left( 1 + x - \frac{ 1 - (1-x)^{n + 1}}{x} \right)
	= \frac{-nx(1-x)^n - (1-x)^n + x^2 + 1}{x^2}
\]


\end{document}